ring tactic with coeffs / powers modulus

src/ecAlgTactic.ml
@@ -32,6 +32,8 @@ module Axioms = struct
   let div   = "div"
   let expr  = "expr"
   let embed = "ofint"
+  let cN    = "Cn"
+  let cP    = "Cp"
 
   let core_add  = ["oner_neq0"; "addr0"; "addrA"; "addrC";]
   let core_mul  = [ "mulr1"; "mulrA"; "mulrC"; "mulrDl"]
@@ -44,27 +46,31 @@ module Axioms = struct
   let ofsub     = ["subrE"]
   let field     = ["mulrV"; "exprN"]
   let ofdiv     = ["divrE"]
+  let cNax      = ["Cn_eq0"]
+  let cPax      = ["Cp_idp"]
 
   let ty0 ty = ty
   let ty1 ty = tfun ty (ty0 ty)
   let ty2 ty = tfun ty (ty1 ty)
 
-  let ring_symbols env boolean ty =
+  let ring_symbols env kind ty =
+    let reqopp = not (kind = `Boolean) in
+
     let symbols =
-      [(zero, (true , ty0 ty));
-       (one , (true , ty0 ty));
-       (add , (true , ty2 ty));
-       (opp , (not boolean, ty1 ty));
-       (sub , (false, ty2 ty));
-       (mul , (true , ty2 ty));
-       (expr, (false, toarrow [ty; tint] ty))]
+      [(zero, (true  , ty0 ty));
+       (one , (true  , ty0 ty));
+       (add , (true  , ty2 ty));
+       (opp , (reqopp, ty1 ty));
+       (sub , (false , ty2 ty));
+       (mul , (true  , ty2 ty));
+       (expr, (false , toarrow [ty; tint] ty))]
     in
       if   EcReduction.EqTest.for_type env ty tint
       then symbols
       else symbols @ [(embed, (false, tfun tint ty))]
 
   let field_symbols env ty =
-    (ring_symbols env false ty)
+    (ring_symbols env `Integer ty)
       @ [(inv, (true , ty1 ty));
          (div, (false, ty2 ty))]
 
@@ -76,7 +82,8 @@ module Axioms = struct
 
     let xpath  = fun x -> EcPath.pqname tmod x in
     let add    = fun subst x p -> EcSubst.add_path subst (xpath x) p in
-    
+    let addctt = fun subst x f -> EcSubst.add_opdef subst (xpath x) ([], f) in
+
     let subst  = 
       EcSubst.add_tydef EcSubst.empty (xpath tname) ([], cr.r_type) in
     let subst  =
@@ -85,11 +92,22 @@ module Axioms = struct
     let subst  = odfl subst (cr.r_sub |> omap (fun p -> add subst sub p)) in
     let subst  = odfl subst (cr.r_exp |> omap (fun p -> add subst expr p)) in
 
-    let subst  = 
-      cr.r_embed |> 
-          (function `Direct | `Default -> subst | `Embed p -> add subst embed p)
+    let subst  =
+      match cr.r_kind with
+      | `Boolean | `Integer -> subst
+      | `Modulus (c, p) ->
+          let subst = odfl subst (c |> omap (fun c -> addctt subst cN (e_int c))) in
+          let subst = odfl subst (p |> omap (fun p -> addctt subst cP (e_int p))) in
+          subst
     in
-      subst
+
+    let subst  = 
+      match cr.r_embed with
+      | `Direct | `Default -> subst
+      | `Embed p -> add subst embed p
+    in
+
+    subst
 
   let subst_of_field (cr : field) =
     let xpath  = fun x -> EcPath.pqname tmod x in
@@ -115,26 +133,36 @@ module Axioms = struct
     in
       List.map for1 axs
 
-  let getr env cr axs = get (`Ring cr) env axs
+  let getr env cr axs = get (`Ring  cr) env axs
   let getf env cr axs = get (`Field cr) env axs 
 
   let ring_axioms env (cr : ring) =
     let axcore = 
-      if cr.r_bool then getr env cr core_bool
-      else getr env cr core in
-    let axint  = 
+      match cr.r_kind with
+      | `Boolean   -> getr env cr core_bool
+      | `Integer   -> getr env cr core
+      | `Modulus _ -> getr env cr core in
+    let axint =
       match cr.r_embed with 
       | `Direct | `Default -> [] | `Embed _ -> getr env cr ofint in
     let axopp = 
       match cr.r_opp with
-      | Some _ when cr.r_bool -> getr env cr ofoppbool
+      | Some _ when cr.r_kind = `Boolean -> getr env cr ofoppbool
       | _ -> [] in
-    let axsub  = 
+    let axsub = 
       match cr.r_sub with None -> [] | Some _ -> getr env cr ofsub in
-    let axexp  = 
+    let axexp = 
       match cr.r_exp with None -> [] | Some _ -> getr env cr intpow in
+    let axCnp =
+      match cr.r_kind with
+      | `Boolean | `Integer -> []
 
-    List.flatten [axcore; axopp; axexp; axint; axsub]
+      | `Modulus (c, p) ->
+            (odfl [] (c |> omap (fun _ -> getr env cr cNax)))
+          @ (odfl [] (p |> omap (fun _ -> getr env cr cPax)))
+    in
+
+    List.flatten [axcore; axopp; axexp; axint; axsub; axCnp]
 
   let field_axioms env (cr : field) =
     let axring = ring_axioms env cr.f_ring in
@@ -182,17 +210,18 @@ let t_ring_congr (cr:cring) (rm:RState.rstate) pe li lv tc =
     f_eq r1 r2 in 
   let r = ring_of_cring cr in
   let f = ofring r rm pe in
-  let f' = ofring r rm' pe in
+  let f'= ofring r rm' pe in
   let concl = FApi.tc1_goal tc in
-  if not (f_equal (f_eq f f') concl) then raise InvalidGoalShape;
-  let sg = List.map mk_goal li in
-  FApi.xmutate1 tc `Ring_congr sg 
+  if   not (f_equal (f_eq f f') concl)
+  then raise InvalidGoalShape
+  else FApi.xmutate1 tc `Ring_congr (List.map mk_goal li)
 
+(* -------------------------------------------------------------------- *)
 let t_field_simplify r eqs (f1, f2) tc =
   let hyps = FApi.tc1_hyps tc in
   let cr = cfield_of_field r in
-  let (c1, n1, d1) = field_simplify hyps cr eqs f1 in
-  let (c2, n2, d2) = field_simplify hyps cr eqs f2 in
+  let (c1, (n1, d1)) = field_simplify hyps cr eqs f1 in
+  let (c2, (n2, d2)) = field_simplify hyps cr eqs f2 in
 
   let c = List.map (fun f -> f_not (f_eq f (emb_fzero r))) (c1 @ c2) in
   let f = f_eq (fdiv r n1 d1) (fdiv r n2 d2) in
@@ -202,7 +231,7 @@ let t_field_simplify r eqs (f1, f2) tc =
 let t_field r eqs (f1, f2) tc =
   let hyps = FApi.tc1_hyps tc in
   let cr = cfield_of_field r in
-  let (c, (n1, n2), (d1, d2)) = field_eq hyps cr eqs f1 f2 in
+  let (c, ((n1, n2), (d1, d2))) = field_eq hyps cr eqs f1 f2 in
   let c  = List.map (fun f -> f_not (f_eq f (emb_fzero r))) c in
   let c  = Sf.elements (Sf.of_list c) in
   let r1 = fmul r n1 d2
@@ -221,10 +250,10 @@ let t_field_congr (cr:cfield) (rm:RState.rstate) pe li lv tc =
     let r2 = oget (RState.get i rm') in
     EcReduction.EqTest.for_type_exn env r1.f_ty r2.f_ty;
     f_eq r1 r2 in 
-  let r = field_of_cfield cr in
-  let f = offield r rm pe in
+  let r  = field_of_cfield cr in
+  let f  = offield r rm pe in
   let f' = offield r rm' pe in
   let concl = FApi.tc1_goal tc in
-  if not (f_equal (f_eq f f') concl) then raise InvalidGoalShape;
-  let sg = List.map mk_goal li in
-  FApi.xmutate1 tc `Field_congr sg 
+  if   not (f_equal (f_eq f f') concl)
+  then raise InvalidGoalShape
+  else FApi.xmutate1 tc `Field_congr (List.map mk_goal li)
