src/ecAlgTactic.mli
@@ -13,19 +13,24 @@ open EcCoreGoal
 val is_module_loaded : EcEnv.env -> bool
 
 (* -------------------------------------------------------------------- *)
-val ring_symbols  : EcEnv.env -> bool -> ty -> (symbol * (bool * ty)) list
+val ring_symbols  : EcEnv.env -> EcDecl.rkind -> ty -> (symbol * (bool * ty)) list
 val field_symbols : EcEnv.env -> ty -> (symbol * (bool * ty)) list
 
 val ring_axioms  : EcEnv.env -> ring  -> (symbol * form) list
 val field_axioms : EcEnv.env -> field -> (symbol * form) list
 
 (* -------------------------------------------------------------------- *)
-val t_ring : ring -> eqs -> form * form -> FApi.backward
-val t_ring_simplify : ring -> eqs -> form * form -> FApi.backward
-val t_ring_congr : cring -> RState.rstate ->
-           EcRing.pexpr -> int list -> form list -> FApi.backward 
+val t_ring : ring -> eq list -> form * form -> FApi.backward
+val t_ring_simplify : ring -> eq list -> form * form -> FApi.backward
 
-val t_field : field -> eqs -> form * form -> FApi.backward
-val t_field_simplify : field -> eqs -> form * form -> FApi.backward
-val t_field_congr : cfield -> RState.rstate ->
-           EcField.fexpr -> int list -> form list -> FApi.backward 
+val t_ring_congr :
+     cring -> RState.rstate -> EcRing.pexpr -> int list
+  -> form list -> FApi.backward 
+
+(* -------------------------------------------------------------------- *)
+val t_field : field -> eq list -> form * form -> FApi.backward
+val t_field_simplify : field -> eq list -> form * form -> FApi.backward
+
+val t_field_congr :
+     cfield -> RState.rstate -> EcField.fexpr -> int list
+  -> form list -> FApi.backward 
