src/ecParsetree.ml
@@ -603,6 +603,7 @@ type ptycinstance = {
   pti_type : (psymbol * pqsymbol list) list * pty;
   pti_ops  : (psymbol * (pty list * pqsymbol)) list;
   pti_axs  : (psymbol * ptactic_core) list;
+  pti_args : [`Ring of (int option * int option)] option;
 }
 
 (* -------------------------------------------------------------------- *)
