src/ecThCloning.ml
@@ -618,7 +618,7 @@ let clone (scenv : EcEnv.env) (thcl : theory_cloning) =
                     | `Default -> `Default
                     | `Embed p -> `Embed (forpath p)
                     end;
-                  r_bool = cr.r_bool; }
+                  r_kind = cr.r_kind; }
 
               and dofield cr =
                 { f_ring = doring cr.f_ring;
